Ordered_Resolution_Prover/Executable_FO_Ordered_Resolution_Prover.thy
@@ -16,7 +16,7 @@ begin
 global_interpretation RP: deterministic_FO_resolution_prover where
   S = "\<lambda>_. {#}" and
   subst_atm = "op \<cdot>" and
-  id_subst = "Var :: _ \<Rightarrow> ('f :: weighted, nat) term" and
+  id_subst = "Var :: _ \<Rightarrow> ('f :: {weighted, compare}, nat) term" and
   comp_subst = "op \<circ>\<^sub>s" and
   renamings_apart = renamings_apart and
   atm_of_atms = "Fun undefined" and
@@ -44,6 +44,9 @@ global_interpretation RP: deterministic_FO_resolution_prover where
   and subsume = RP.subsume
   and weight = RP.weight
   and St0 = RP.St0
+  and sorted_list_of_set = "linorder.sorted_list_of_set (le_of_comp compare)"
+  and sort_key = "linorder.sort_key (le_of_comp compare)"
+  and insort_key = "linorder.insort_key (le_of_comp compare)"
   by (unfold_locales)
     (auto simp: less_kbo_subst is_ground_atm_ground less_kbo_less intro: ground_less_less_kbo)
 
@@ -65,22 +68,29 @@ declare
   substitution_ops.subst_lit_def[code]
   substitution_ops.subst_cls_def[code]
 
-lemma [code]: "mgu_sets = mgu_sets"
-  by simp
-
 lemma [code]: "is_reducible_lit = is_reducible_lit"
   by simp
 
 lemma [code]: "substitution_ops.subsumes = substitution_ops.subsumes"
   by simp
 
+declare
+  Pairs_def[folded sorted_list_of_set_def, code]
+  linorder.sorted_list_of_set_sort_remdups[OF class_linorder_compare,
+    folded sorted_list_of_set_def sort_key_def, code]
+  linorder.sort_key_def[OF class_linorder_compare, folded sort_key_def insort_key_def, code]
+  linorder.insort_key.simps[OF class_linorder_compare, folded insort_key_def, code]
+
 export_code St0 in SML
-export_code deterministic_RP in SML
+export_code deterministic_RP in SML module_name RP
 
 definition prover where
   "prover N = deterministic_RP (St0 N 0)"
 
-export_code prover in SML
+lemma "prover N = None \<Longrightarrow> satisfiable (RP.grounded_N0 N)"
+  unfolding prover_def St0_def by (rule RP.deterministic_RP_complete)
+
+export_code prover in SML module_name RP
 
 value "prover ([] :: ((unit, nat) Term.term literal list \<times> nat) list)"
 
